'wf' includes term 'x'

App/Lib/NatRangeIterator/Spec.v
@@ -8,14 +8,15 @@ Import ObjectOrientedNotations.
 Section Specs.
 Open Scope oo_scope.
 
-Definition wf_ex (var : tm) (st : state) : Prop :=
-  exists n ref at_start count first,
-      var = tvar n
-  /\  read_sk_hd n st = tref ref
+Definition wf_ex (x : tm) (st : state) : Prop :=
+  exists var ref at_start count first,
+      x = tvar var
+  /\  read_sk_hd var st = tref ref
   /\  read_sr ref st = tcl "NatRangeIterator" <(tbool at_start, tnat count, tnat first)>.
 
-Definition wf var ref st at_start count first : Prop :=
-      read_sk_hd var st = tref ref
+Definition wf x var ref st at_start count first : Prop :=
+      x = tvar var
+  /\  read_sk_hd var st = tref ref
   /\  read_sr ref st = tcl "NatRangeIterator" <(tbool at_start, tnat count, tnat first)>.
 
 Variable step : step_relation.
@@ -27,9 +28,9 @@ Notation "t1 '/' st1 '==>*' t2 '/' st2" := (multi step (pair t1 st1) (pair t2 st
   (at level 40, st1 at level 39, t2 at level 39, format "'[' t1 / st1 '==>*' t2 / st2 ']'").
 
 Definition get_at_start__behavior : Prop :=
-  forall var ref st at_start count first,
-  wf var ref st at_start count first ->
-  ((tvar var) # "get_at_start"|()|) / st ==>* (tbool at_start) / st.
+  forall x var ref st at_start count first,
+  wf x var ref st at_start count first ->
+  (x # "get_at_start"|()|) / st ==>* (tbool at_start) / st.
 
 Definition get_at_start__returns_tbool : Prop :=
   forall v x st st',
